equivalence.dfy
@@ -7,64 +7,68 @@ module Equivalence{
     // import opened Lemmas
     import opened Common
     import opened Steps
-    ghost predicate AreEquivalent(bf_program: Program, bf_state: State, ir_program: IntermediateRep, input: seq<char>, inputPtr: int)
-    requires 0 <= bf_program.pointer <= |bf_program.commands|
-    requires 0 <= bf_state.pointer < |bf_state.memory| 
-    decreases |bf_program.commands|- bf_program.pointer
-    requires 0 <= inputPtr <= |input|
-    requires valid_program(bf_program) 
-    requires state_reqs(bf_state)
-    ensures !(bf_program.pointer >= |bf_program.commands| && !(ir_program.pointer >= |ir_program.commands|)) || !(!(bf_program.pointer >= |bf_program.commands|) && (ir_program.pointer >= |ir_program.commands|))
-        {
-            if bf_program.pointer >= |bf_program.commands| && ir_program.pointer >= |ir_program.commands| then
-                true
-            else if !(bf_program.pointer >= |bf_program.commands| && !(ir_program.pointer >= |ir_program.commands|)) || !(!(bf_program.pointer >= |bf_program.commands|) && (ir_program.pointer >= |ir_program.commands|)) then
-            // else 
-                // exists i: int :: true
-                // true
-                exists next_bf_state: State, next_bf_program: Program, next_ir: IntermediateRep, postPtr: int:: 
-                0<=bf_program.pointer < next_bf_program.pointer <= |next_bf_program.commands| &&
-                0 <= ir_program.pointer < next_ir.pointer <= |ir_program.commands| &&
-                inputPtr <= postPtr <= |input| &&
+    // ghost predicate AreEquivalent(bf_program: Program, bf_state: State, ir_program: IntermediateRep, input: seq<char>, inputPtr: int)
+    // requires 0 <= bf_program.pointer <= |bf_program.commands|
+    // requires 0 <= bf_state.pointer < |bf_state.memory| 
+    // decreases |bf_program.commands|- bf_program.pointer
+    // requires 0 <= inputPtr <= |input|
+    // requires valid_program(bf_program) 
+    // requires state_reqs(bf_state)
+    // ensures !(bf_program.pointer >= |bf_program.commands| && !(ir_program.pointer >= |ir_program.commands|)) || !(!(bf_program.pointer >= |bf_program.commands|) && (ir_program.pointer >= |ir_program.commands|))
+    //     {
+    //         if bf_program.pointer >= |bf_program.commands| && ir_program.pointer >= |ir_program.commands| then
+    //             true
+    //         else if !(bf_program.pointer >= |bf_program.commands| && !(ir_program.pointer >= |ir_program.commands|)) || !(!(bf_program.pointer >= |bf_program.commands|) && (ir_program.pointer >= |ir_program.commands|)) then
+    //         // else 
+    //             // exists i: int :: true
+    //             // true
+    //             exists next_bf_state: State, next_bf_program: Program, next_ir: IntermediateRep, postPtr: int:: 
+    //             0<=bf_program.pointer < next_bf_program.pointer <= |next_bf_program.commands| &&
+    //             0 <= ir_program.pointer < next_ir.pointer <= |ir_program.commands| &&
+    //             inputPtr <= postPtr <= |input| &&
 
-                next_ir.commands == ir_program.commands && bf_program.commands == next_bf_program.commands
-                &&
-                state_reqs(next_bf_state)
-                &&
-                |next_bf_state.memory| == |bf_state.memory|
-                // &&
-                && 0<=next_bf_state.pointer < |next_bf_state.memory| 
-                && max_steps(bf_program, bf_state, next_bf_program, next_bf_state)
-                && ir_step(ir_program, bf_state, next_ir, next_bf_state) && AreEquivalent(next_bf_program, next_bf_state, next_ir, input, postPtr)
+    //             next_ir.commands == ir_program.commands && bf_program.commands == next_bf_program.commands
+    //             &&
+    //             state_reqs(next_bf_state)
+    //             &&
+    //             |next_bf_state.memory| == |bf_state.memory|
+    //             // &&
+    //             && 0<=next_bf_state.pointer < |next_bf_state.memory| 
+    //             && max_steps(bf_program, bf_state, next_bf_program, next_bf_state)
+    //             && ir_step(ir_program, bf_state, next_ir, next_bf_state) && AreEquivalent(next_bf_program, next_bf_state, next_ir, input, postPtr)
             
-            else
-                false 
-        }
+    //         else
+    //             false 
+    //     }
 
-
+    ghost predicate equiv_locations(p: Program, ir: IntermediateRep)
+    {
+        (ir.pointer == |ir.commands| && p.pointer == |p.commands|) || (0<= ir.pointer < |Changes(p)| && p.pointer == Changes(p)[ir.pointer])
+    }
     ghost predicate EquivalentReps(p: Program, s: State, ir: IntermediateRep)
     requires valid_program(p)
     requires state_reqs(s)
     requires valid_ir(ir)
     requires valid_input(ir.input) 
     {
-        //Idea: forall values, from any linear location in the program or in the code, they should transition to the same spot
-        // Will call this from any state as well
-(        forall i:: within_ir_range(i, ir) ==> exists p': Program, s': State, ir': IntermediateRep, s1: State:: valid_program(p') && aligned_programs(p, p') && valid_state(s, s') && state_reqs(s')  && program_k_max_steps(p, s, p', s', i) && state_reqs(s1) && valid_state(s, s1) && valid_ir(ir') && valid_input(ir'.input) && ir_step(IntermediateRep(ir.commands, i, ir.input), s, ir', s1) && s'==s1 )
+        //For all values, from any linear location in the program or in the code, 
+        //they should transition to the same spot
+        (forall i:: within_ir_range(i, ir) ==> exists p': Program, s': State, ir': IntermediateRep, s1: State:: 
+        valid_program(p') && aligned_programs(p, p') && valid_state(s, s') && state_reqs(s')  && 
+        program_k_max_steps(p, s, p', s', i) 
+        && state_reqs(s1) && valid_state(s, s1) && valid_ir(ir') && valid_input(ir'.input) && 
+        ir_step(IntermediateRep(ir.commands, i, ir.input), s, ir', s1) 
+        && s'==s1)
     }
 
-    ghost predicate lockstep(p: Program, s: State, ir: IntermediateRep)
+    ghost predicate FullEquivalence(p: Program, ir: IntermediateRep)
     requires valid_program(p)
-    requires state_reqs(s)
     requires valid_ir(ir)
     requires valid_input(ir.input)
     {
-        valid_program(p) && valid_ir(ir) && state_reqs(s) &&
-        exists p': Program, s': State, ir': IntermediateRep ::
-        valid_program(p') && state_reqs(s')&& valid_ir(ir')&& valid_input(ir'.input)&& valid_state(s, s')&& aligned_programs(p, p') &&
-        max_steps( p, s, p', s') &&
-        ir_step(ir, s, ir', s')     
+        forall s: State:: state_reqs(s) ==> EquivalentReps(p, s, ir)
     }
+
 
 ghost predicate matched_forall_loop(p: Program, ir: seq<Instr>, changes: seq<int>, bound: int)
 requires valid_program(p)
@@ -93,7 +97,18 @@ match ir[index]
         ((k>= 0 ==> ((p.commands[changes[index]]=='>') && k==count_consecutive_symbols(p, changes[index]))) && (k<0 ==> (p.commands[changes[index]]=='<')&&(-k)==count_consecutive_symbols(p, changes[index])))
     case UserInput => p.commands[changes[index]] == ','
     case Print => p.commands[changes[index]] == '.'
-    case Jump(dest, direction) => ((p.commands[changes[index]] == ']' && direction == false) || (p.commands[changes[index]] == '[' && direction == true))
+    case Jump(dest, false) => (
+        (p.commands[changes[index]] == ']')
+        // && p.commands[changes[dest]] == '[' && ir[dest] == Jump(index, true))
+        // && valid_loop(p.commands[changes[dest]+1.. changes[index]])
+        )
+    case Jump(dest, true)=>
+         (
+            p.commands[changes[index]] == '['
+            
+            )
+            
+    
 }
 
 ghost predicate aligned_instructions_subseq(p: Program, ir: seq<Instr>)
