loops.dfy
@@ -1,0 +1,650 @@
+include "lemmas.dfy"
+include "common.dfy"
+include "steps.dfy"
+include "equivalence.dfy"
+include "triviallemmas.dfy"
+
+
+
+module Loops {
+import opened Lemmas
+import opened Common
+import opened Steps
+import opened Equivalence
+import opened Trivial
+
+predicate valid_loop_ir(ir: IntermediateRep)
+{
+    valid_loop_ir_helper(ir.commands, 0, 0)
+}
+
+predicate valid_loop_ir_helper(ir: seq<Instr>, balance: int, i: int)
+requires 0<=i<=|ir|
+decreases |ir|-i
+{
+if |ir| == i then
+    balance == 0
+else 
+    match ir[i]
+        case Jump(k, true) => valid_loop_ir_helper(ir, balance + 1, i+1)
+        case Jump(k, false) => balance > 0 && valid_loop_ir_helper(ir, balance - 1, i+1)
+        case _ => valid_loop_ir_helper(ir, balance, i+1)
+}
+// predicate valid_loop_program(p: seq<char>)
+
+// {
+//     empty_body(p) || 
+//     (
+//         forall i:: (0<= i < |p| ==>(
+//             (p[i]== '[' ==> exists k::  i< k < |p| && p[k]== ']' && valid_loop_program(p[i+1..k]))
+//             &&
+//             (p[i]== ']' ==> exists k::  0<= k < i && p[k]== '[' && valid_loop_program(p[k+1..i]))
+//         ))
+//     )
+// }
+// predicate loop_pred(p: seq<char>, i: int)
+// requires 0 <= i < |p|
+// {
+//     (p[i]== '[' ==> exists k::  i< k < |p| && p[k]== ']' && valid_loop_program(p[i+1..k]))
+//         &&
+//     (p[i]== ']' ==> exists k::  0<= k < i && p[k]== '[' && valid_loop_program(p[k+1..i]))
+// }
+
+// predicate loop_pred_ir(ir: seq<Instr>, i: int)
+// requires 0<= i < |ir|
+// {
+//     (match ir[i]
+//         case Jump(j, true) =>
+//             (exists k:: i< k < |ir| && (
+//                 match ir[k]
+//                     case Jump(_, false) => true
+//                     case _ => false
+//             ) && valid_loop_ir(ir[i+1..k]))
+//         case Jump(j, false) => (
+//             exists k:: 0 <= k < i && (
+//                 match ir[k] 
+//                     case Jump(_, true) => true
+//                     case _ => false
+//             ) && valid_loop_ir(ir[k+1..i])
+//         )
+//         case _ => true
+        
+//     )
+// }
+
+// predicate valid_loop_ir(ir: seq<Instr>)
+
+// {
+//     |ir| == 0 || 
+//     (
+//         forall i:: (0<= i < |ir| ==>( loop_pred_ir(ir, i)
+//             // (match ir[i]
+//             //     case Jump(j, true) =>
+//             //         (exists k:: i< k < |ir| && (
+//             //             match ir[k]
+//             //                 case Jump(_, false) => true
+//             //                 case _ => false
+//             //         ) && valid_loop_ir(ir[i+1..k]))
+//             //     case Jump(j, false) => (
+//             //         exists k:: 0 <= k < i && (
+//             //             match ir[k] 
+//             //                 case Jump(_, true) => true
+//             //                 case _ => false
+//             //         ) && valid_loop_ir(ir[k+1..i])
+//             //     )
+//             //     case _ => true
+                
+//             // )
+//         ))
+//     )
+// }
+
+lemma aligned_implies_valid(p: Program, ir: IntermediateRep)
+requires valid_loop_program(p)
+requires valid_ir(ir)
+requires valid_program(p)
+requires aligned_instructions(p, ir)
+ensures valid_loop_ir(ir)
+{
+    var indices := Changes(p);
+    ChangeLemma(p, indices);
+    aligned_implies_valid_helper(p, ir, 0, indices, 0, 0);
+    assert valid_loop_ir_helper(ir.commands, 0, 0);
+}
+
+lemma addition_balance(p: Program, balance: int, p_index: int, new_balance: int, new_p: int)
+requires valid_program(p)
+requires 0<= p_index+1 <= |p.commands|
+requires valid_loop_program_helper(p.commands, balance+1, p_index+1)
+requires new_balance == balance+1
+requires new_p == p_index+1
+ensures valid_loop_program_helper(p.commands, new_balance, new_p)
+{}
+
+lemma addition_balance_k(p: Program, balance: int, p_index: int, new_balance: int, new_p: int, k:int)
+requires valid_program(p)
+requires 0<= p_index+k <= |p.commands|
+requires valid_loop_program_helper(p.commands, balance, p_index+k)
+requires new_balance == balance
+requires new_p == p_index+k
+ensures valid_loop_program_helper(p.commands, new_balance, new_p)
+{}
+
+lemma subtraction_balance(p: Program, balance: int, p_index: int, new_balance: int, new_p: int)
+requires valid_program(p)
+requires 0<= p_index+1 <= |p.commands|
+requires valid_loop_program_helper(p.commands, balance-1, p_index+1)
+requires new_balance == balance-1
+requires new_p == p_index+1
+ensures valid_loop_program_helper(p.commands, new_balance, new_p)
+{}
+
+lemma even_balance(p: Program, balance: int, p_index: int, new_balance: int, new_p: int)
+requires valid_program(p)
+requires 0<= p_index+1 <= |p.commands|
+requires valid_loop_program_helper(p.commands, balance, p_index+1)
+requires new_balance == balance
+requires new_p == p_index+1
+ensures valid_loop_program_helper(p.commands, new_balance, new_p)
+{}
+
+lemma aligned_implies_valid_helper(p: Program, ir: IntermediateRep, balance: int, indices: seq<int>, index: int, p_index: int)
+requires 0 <= index <= |indices|
+requires balance >= 0
+requires indices == Changes(p)
+requires changes_correct(p, indices)
+requires valid_ir(ir)
+requires valid_program(p)
+requires aligned_instructions(p, ir)
+decreases |indices|-index
+requires (index == |indices| && p_index == |p.commands|) || (index < |indices| && p_index == indices[index]) 
+requires valid_loop_program_helper(p.commands, balance, p_index)
+ensures valid_loop_ir_helper(ir.commands, balance, index)
+{
+    if index == |indices|{
+        assert index == |ir.commands|;
+        assert valid_loop_ir_helper(ir.commands, balance, index);
+    }else{
+    var p_index := indices[index];
+        match p.commands[p_index] 
+            case '[' => {
+                // assert balance >=0;
+                // assume false;
+                assert (match ir.commands[index]
+                    case Jump(_, true) => true
+                    case _ => false
+                );
+                // assert ((!(index+1 in indices)&&indices[index]+1 == |p.commands| ) || (indices[index]+1 < |p.commands| && indices[index]+1 in indices));    
+                if index+1 < |indices|{
+                    assert index+1 < |indices|;
+                    assert indices[index+1] == p_index+1;
+                    // assert indices[index+1]
+                }else{
+                    LemmaStrictlyIncreasing(indices);
+                    assert p_index+1 == |p.commands|;
+                }
+                // assume false;
+
+                assert valid_loop_program_helper(p.commands, balance+1, p_index+1);
+                assert 0 <= index+1 <= |indices|;
+                assert indices == Changes(p);
+                assert changes_correct(p, indices);
+                assert valid_ir(ir);
+                assert valid_program(p);
+                assert aligned_instructions(p, ir);
+                assert ( p_index+1 == |p.commands|) || (index+1 < |indices| && p_index+1 == indices[index+1]);
+                var new_b := balance+1;
+                var new_p_ind := p_index+1;
+                var new_ind := index+1;
+                addition_balance(p, balance, p_index, new_b, new_p_ind);
+                assert valid_loop_program_helper(p.commands, new_b, new_p_ind);
+                assert (new_p_ind == |p.commands|) || (new_ind < |indices| && new_p_ind == indices[new_ind]);
+                assert 0 <= new_ind <= |indices|;
+                aligned_implies_valid_helper(p, ir, new_b, indices, new_ind, new_p_ind);
+            }
+            case ']' => {
+                // assume false;
+                assert balance > 0;
+                assert (match ir.commands[index]
+                    case Jump(_, false) => true
+                    case _ => false
+                );
+                if index+1 < |indices|{
+                    assert index+1 < |indices|;
+                    assert indices[index+1] == p_index+1;
+                }else{
+                    // assert 
+                    LemmaStrictlyIncreasing(indices);
+                    assert p_index+1 == |p.commands|;
+                }
+                assert valid_loop_program_helper(p.commands, balance-1, p_index+1);
+                assert 0 <= index+1 <= |indices|;
+                assert indices == Changes(p);
+                assert changes_correct(p, indices);
+                assert valid_ir(ir);
+                assert valid_program(p);
+                assert aligned_instructions(p, ir);
+                assert ( p_index+1 == |p.commands|) || (index+1 < |indices| && p_index+1 == indices[index+1]);
+                var new_b := balance-1;
+                var new_p_ind := p_index+1;
+                var new_ind := index+1;
+                subtraction_balance(p, balance, p_index, new_b, new_p_ind);
+                assert valid_loop_program_helper(p.commands, new_b, new_p_ind);
+                assert (new_p_ind == |p.commands|) || (new_ind < |indices| && new_p_ind == indices[new_ind]);
+                assert 0 <= new_ind <= |indices|;
+                aligned_implies_valid_helper(p, ir, new_b, indices, new_ind, new_p_ind);
+
+                // aligned_implies_valid_helper(p, ir, balance-1, indices, index+1, p_index+1);
+            }
+            case ',' => {
+                assert (match ir.commands[index]
+                    case Jump(_, _) => false
+                    case UserInput => true
+                    case _ => false
+                );
+                if index+1 < |indices|{
+                    assert index+1 < |indices|;
+                    assert indices[index+1] == p_index+1;
+                }else{
+                    // assert 
+                    LemmaStrictlyIncreasing(indices);
+                    assert p_index+1 == |p.commands|;
+                }
+                // assume false;
+                assert valid_loop_program_helper(p.commands, balance, p_index+1);
+                assert 0 <= index+1 <= |indices|;
+                assert indices == Changes(p);
+                assert changes_correct(p, indices);
+                assert valid_ir(ir);
+                assert valid_program(p);
+                assert aligned_instructions(p, ir);
+                assert ( p_index+1 == |p.commands|) || (index+1 < |indices| && p_index+1 == indices[index+1]);
+                var new_p_ind := p_index+1;
+                var new_ind := index+1;
+                var new_b := balance;
+                even_balance(p, balance, p_index, new_b, new_p_ind);
+                assert valid_loop_program_helper(p.commands, new_b, new_p_ind);
+                assert (new_p_ind == |p.commands|) || (new_ind < |indices| && new_p_ind == indices[new_ind]);
+                assert 0 <= new_ind <= |indices|;
+                aligned_implies_valid_helper(p, ir, new_b, indices, new_ind, new_p_ind);
+            }
+            case '.' =>{
+                assert (match ir.commands[index]
+                    case Jump(_, _) => false
+                    case Print => true
+                    case _ => false
+                );
+                if index+1 < |indices|{
+                    assert index+1 < |indices|;
+                    assert indices[index+1] == p_index+1;
+                }else{
+                    // assert 
+                    LemmaStrictlyIncreasing(indices);
+                    assert p_index+1 == |p.commands|;
+                }
+                // assume false;
+                assert valid_loop_program_helper(p.commands, balance, p_index+1);
+                assert 0 <= index+1 <= |indices|;
+                assert indices == Changes(p);
+                assert changes_correct(p, indices);
+                assert valid_ir(ir);
+                assert valid_program(p);
+                assert aligned_instructions(p, ir);
+                assert ( p_index+1 == |p.commands|) || (index+1 < |indices| && p_index+1 == indices[index+1]);
+                var new_p_ind := p_index+1;
+                var new_ind := index+1;
+                var new_b := balance;
+                even_balance(p, balance, p_index, new_b, new_p_ind);
+                assert valid_loop_program_helper(p.commands, new_b, new_p_ind);
+                assert (new_p_ind == |p.commands|) || (new_ind < |indices| && new_p_ind == indices[new_ind]);
+                assert 0 <= new_ind <= |indices|;
+                aligned_implies_valid_helper(p, ir, new_b, indices, new_ind, new_p_ind);
+            }
+            case '>'=>{
+                ValidLoopMoveRight(p, ir, index, p_index, indices);
+                // assert (match ir.commands[index]
+                //     case Jump(_, _) => false
+                //     case _ => true
+                // );
+                var k := count_consecutive_symbols(p, p_index);
+                loop_helper_stays_constant(p, k, p_index, balance, '>');
+                var new_p_ind := p_index+k;
+                var new_b := balance;
+                addition_balance_k(p, balance, p_index, new_b, new_p_ind, k);
+            }
+            case '<'=>{
+                // assume false;
+                ValidLoopMoveLeft(p, ir, index, p_index, indices);
+                // assert (match ir.commands[index]
+                //     case Jump(_, _) => false
+                //     case _ => true
+                // );
+                var k := count_consecutive_symbols(p, p_index);
+                loop_helper_stays_constant(p, k, p_index, balance, '<');
+                var new_p_ind := p_index+k;
+                var new_b := balance;
+                addition_balance_k(p, balance, p_index, new_b, new_p_ind, k);
+            }
+            case '+'=>{
+                // assume false;
+                ValidLoopAdd(p, ir, index, p_index, indices);
+                // assert (match ir.commands[index]
+                //     case Jump(_, _) => false
+                //     case _ => true
+                // );
+                var k := count_consecutive_symbols(p, p_index);
+                loop_helper_stays_constant(p, k, p_index, balance, '+');
+                var new_p_ind := p_index+k;
+                var new_b := balance;
+                addition_balance_k(p, balance, p_index, new_b, new_p_ind, k);
+            }
+            case '-'=>{
+                // assume false;
+                ValidLoopSub(p, ir, index, p_index, indices);
+                // assert (match ir.commands[index]
+                //     case Jump(_, _) => false
+                //     case _ => true
+                // );
+                var k := count_consecutive_symbols(p, p_index);
+                loop_helper_stays_constant(p, k, p_index, balance, '-');
+                var new_p_ind := p_index+k;
+                var new_b := balance;
+                addition_balance_k(p, balance, p_index, new_b, new_p_ind, k);
+            }
+            case _ => {
+                assume false;
+            }
+    }
+}
+
+lemma ValidLoopMoveRight (p: Program, ir: IntermediateRep, index: int, p_index: int, indices: seq<int>)
+requires valid_program(p)
+requires valid_ir(ir)
+requires 0 <= index < |indices|
+requires p_index == indices[index]
+requires indices == Changes(p)
+requires changes_correct(p, indices)
+requires aligned_instructions(p, ir)
+requires p.commands[p_index] == '>'
+ensures (p_index+count_consecutive_symbols(p, p_index) == |p.commands|) 
+    || (index+1 < |indices| && p_index+count_consecutive_symbols(p, p_index) == indices[index+1])
+ensures (match ir.commands[index]
+                    case Jump(_, _) => false
+                    case _ => true
+                )
+{
+    assert matched_command_with_ir(p, ir.commands, index, indices);
+    assert (match ir.commands[index]
+            case Jump(dest, true) =>
+                p.commands[indices[index]] == '['
+            case Jump(dest, false) => (
+                p.commands[indices[index]] == ']'
+            )
+            case _ => true
+        );
+    var k := count_consecutive_symbols(p, p_index);
+    if index+1 < |indices|{
+        assert index+1 < |indices|;
+        assert indices[index+1] == p_index+k;
+    }else{
+        // assert 
+        LemmaStrictlyIncreasing(indices);
+        assert p_index+k == |p.commands|;
+    }
+}
+lemma ValidLoopMoveLeft (p: Program, ir: IntermediateRep, index: int, p_index: int, indices: seq<int>)
+requires valid_program(p)
+requires valid_ir(ir)
+requires 0 <= index < |indices|
+requires p_index == indices[index]
+requires indices == Changes(p)
+requires changes_correct(p, indices)
+requires aligned_instructions(p, ir)
+requires p.commands[p_index] == '<'
+ensures (p_index+count_consecutive_symbols(p, p_index) == |p.commands|) 
+    || (index+1 < |indices| && p_index+count_consecutive_symbols(p, p_index) == indices[index+1])
+ensures (match ir.commands[index]
+                    case Jump(_, _) => false
+                    case _ => true
+                )
+{
+    assert matched_command_with_ir(p, ir.commands, index, indices);
+    assert (match ir.commands[index]
+            case Jump(dest, true) =>
+                p.commands[indices[index]] == '['
+            case Jump(dest, false) => (
+                p.commands[indices[index]] == ']'
+            )
+            case _ => true
+        );
+    var k := count_consecutive_symbols(p, p_index);
+    if index+1 < |indices|{
+        assert index+1 < |indices|;
+        assert indices[index+1] == p_index+k;
+    }else{
+        // assert 
+        LemmaStrictlyIncreasing(indices);
+        assert p_index+k == |p.commands|;
+    }
+}
+
+lemma ValidLoopAdd (p: Program, ir: IntermediateRep, index: int, p_index: int, indices: seq<int>)
+requires valid_program(p)
+requires valid_ir(ir)
+requires 0 <= index < |indices|
+requires p_index == indices[index]
+requires indices == Changes(p)
+requires changes_correct(p, indices)
+requires aligned_instructions(p, ir)
+requires p.commands[p_index] == '+'
+ensures (p_index+count_consecutive_symbols(p, p_index) == |p.commands|) 
+    || (index+1 < |indices| && p_index+count_consecutive_symbols(p, p_index) == indices[index+1])
+ensures (match ir.commands[index]
+                    case Jump(_, _) => false
+                    case _ => true
+                )
+{
+    assert matched_command_with_ir(p, ir.commands, index, indices);
+    assert (match ir.commands[index]
+            case Jump(dest, true) =>
+                p.commands[indices[index]] == '['
+            case Jump(dest, false) => (
+                p.commands[indices[index]] == ']'
+            )
+            case _ => true
+        );
+    var k := count_consecutive_symbols(p, p_index);
+    if index+1 < |indices|{
+        assert index+1 < |indices|;
+        assert indices[index+1] == p_index+k;
+    }else{
+        // assert 
+        LemmaStrictlyIncreasing(indices);
+        assert p_index+k == |p.commands|;
+    }
+}
+
+lemma ValidLoopSub (p: Program, ir: IntermediateRep, index: int, p_index: int, indices: seq<int>)
+requires valid_program(p)
+requires valid_ir(ir)
+requires 0 <= index < |indices|
+requires p_index == indices[index]
+requires indices == Changes(p)
+requires changes_correct(p, indices)
+requires aligned_instructions(p, ir)
+requires p.commands[p_index] == '-'
+ensures (p_index+count_consecutive_symbols(p, p_index) == |p.commands|) 
+    || (index+1 < |indices| && p_index+count_consecutive_symbols(p, p_index) == indices[index+1])
+ensures (match ir.commands[index]
+                    case Jump(_, _) => false
+                    case _ => true
+                )
+{
+    assert matched_command_with_ir(p, ir.commands, index, indices);
+    assert (match ir.commands[index]
+            case Jump(dest, true) =>
+                p.commands[indices[index]] == '['
+            case Jump(dest, false) => (
+                p.commands[indices[index]] == ']'
+            )
+            case _ => true
+        );
+    var k := count_consecutive_symbols(p, p_index);
+    if index+1 < |indices|{
+        assert index+1 < |indices|;
+        assert indices[index+1] == p_index+k;
+    }else{
+        // assert 
+        LemmaStrictlyIncreasing(indices);
+        assert p_index+k == |p.commands|;
+    }
+}
+
+
+predicate less_than_k(j: int, k: int)
+{
+    (0<=j<k)
+}
+
+lemma loop_helper_stays_constant (p: Program, k: int, p_index: int, balance: int, c: char)
+requires 0<= p_index < |p.commands|
+requires k >0
+requires p_index+k <= |p.commands|
+requires c == '>' || c == '<' || c == '+' || c== '-'
+requires valid_loop_program_helper(p.commands, balance, p_index)
+requires forall j:: less_than_k(j, k) ==> p.commands[p_index+j] == c
+ensures valid_loop_program_helper(p.commands, balance, p_index+k)
+{
+    var i := 0;
+    while i < k
+    invariant i<=k
+    invariant valid_loop_program_helper(p.commands, balance, p_index+i)
+    {
+        assert valid_loop_program_helper(p.commands, balance, p_index+i);
+        assert less_than_k(i, k);
+        assert p.commands[p_index+i]==c;
+        assert valid_loop_program_helper(p.commands, balance, p_index+i+1);
+        i := i+1;
+        assert valid_loop_program_helper(p.commands, balance, p_index+i);
+    }
+    assert i==k;
+    assert valid_loop_program_helper(p.commands, balance, p_index+i);
+}
+
+predicate valid_loop_program(p: Program)
+{
+    valid_loop_program_helper(p.commands, 0, 0)
+}
+
+predicate valid_loop_program_helper(p: seq<char>, balance: int, i: int)
+requires 0<=i <= |p|
+decreases |p|-i
+{
+if i == |p| then
+    balance == 0
+  else if p[i] == '[' then
+    valid_loop_program_helper(p, balance + 1, i+1)
+  else if p[i] == ']' then
+    balance > 0 && valid_loop_program_helper(p, balance - 1, i+1)
+  else
+    valid_loop_program_helper(p, balance, i+1)
+}
+predicate non_merge_symbols(p: Program, res: seq<int>)
+{
+    forall i:: (0<=i<|p.commands| && (p.commands[i] == '[' || p.commands[i] == ']' || p.commands[i] == '.' || p.commands[i] == ',') 
+    ==> (exists k:: 0<= k < |Changes(p)| && Changes(p)[k]==i))
+}
+predicate non_merged_aligned_helper(p: Program, ir: IntermediateRep, i: int)
+requires 0 <= i < |p.commands|
+requires |ir.commands| == |Changes(p)|
+{
+    
+    exists k :: (0 <= k < |ir.commands| &&
+    (match p.commands[i]
+        case '[' =>
+            (match ir.commands[k]
+                case Jump(x, true) => true
+                case _ => false
+            )&& Changes(p)[k] == i
+        case ']' =>
+            (match ir.commands[k]
+                case Jump(x, false) => true
+                case _ => false
+            )&& Changes(p)[k] == i
+        case '.' =>
+            (match ir.commands[k]
+                case Print => true
+                case _ => false
+            )&& Changes(p)[k] == i
+        case ',' =>
+            (match ir.commands[k]
+                case UserInput => true
+                case _ => false
+            )&& Changes(p)[k] == i
+        case _ => true
+
+    ))
+}
+predicate non_merged_aligned(p: Program, ir: IntermediateRep)
+requires |ir.commands| == |Changes(p)|
+{
+    forall i:: (0 <= i < |p.commands| ==>
+        non_merged_aligned_helper(p, ir, i)
+    )
+}
+
+predicate subRepSubProgram(p: Program, ir: IntermediateRep, startProgram: int, startIR: int, endProgram: int, endIR: int,
+p': Program, ir': IntermediateRep)
+requires |Changes(p)| == |ir.commands|
+{
+    0 <= startProgram < endProgram < |p.commands|
+    && 0<= startIR < endIR < |ir.commands|
+    && Changes(p)[startIR] == startProgram
+    && Changes(p)[endIR] == endProgram
+    && p' == Program(p.commands[startProgram+1.. endProgram], 0, p.input)
+    && ir' == IntermediateRep(ir.commands[startIR+1..endIR], 0, ir.input)
+}
+
+
+
+lemma strictlyIncreasing (s: seq<int>, i: int, j: int)
+requires |s| > 0
+requires strictly_increasing(s)
+requires 0 <= i < |s|
+requires 0 <= j < |s|
+ensures s[i] < s[j] ==> i < j
+{}
+
+
+
+ 
+
+method Compile(p: Program)  returns (result: IntermediateRep)
+  requires valid_program(p)
+  requires valid_loop_program(p)
+  requires |p.commands| > 0
+  ensures true
+
+{
+    var i := 0;
+    var commands := [];
+
+    while i < |p.commands|
+    decreases |p.commands|-i
+    {
+        {match p.commands[i]
+            case '[' => {
+                commands := commands + [Jump(0, true)];
+            }
+            case ']' => {
+                commands := commands + [Jump(0, false)];
+            }
+            case _ => {
+                commands := commands + [Print];
+            }
+        }
+        i := i+1;
+    }
+    result := IntermediateRep(commands, 0, p.input);
+}
+}
