triviallemmas.dfy
@@ -1,0 +1,192 @@
+include "common.dfy"
+include "steps.dfy"
+include "equivalence.dfy"
+
+module Trivial{
+    import opened Common 
+    import opened Steps
+    import opened Equivalence
+
+    lemma IndexedImpliesMembership(s: seq<int>)
+        ensures forall d :: 0 <= d < |s| ==> s[d] in s
+    {}
+
+    lemma EqualIndex(p: seq<char>, k: int, i: int)
+        requires 0<= k < |p|
+        requires i-1 == k
+        ensures p[i-1]==p[k]
+    {}
+
+    lemma AndIsImplicationMoveBackwards(p: Program, ir: seq<Instr>, index: int, changes: seq<int>, k: int)
+        requires valid_program(p)
+        requires changes == Changes(p)
+        requires 0<= index < |ir|
+        requires 0<= index < |changes|
+        requires 0<= changes[index] < |p.commands|
+        requires forall d:: 0<= d < |changes| ==> 0<= changes[d] < |p.commands|
+        requires p.commands[changes[index]] == '<'
+        requires k == -1*count_consecutive_symbols(p, changes[index])
+        requires matched_forall_loop(p, ir, changes, index)
+        requires k < 0
+        requires ir[index] == Move(k)
+        ensures matched_command_with_ir(p, ir, index, changes)
+        ensures matched_forall_loop(p, ir, changes, index+1)
+    {}
+
+    lemma AndIsImplicationJumpFor(p: Program, ir: seq<Instr>, index: int, changes: seq<int>, dest: int)
+        requires valid_program(p)
+        requires changes == Changes(p)
+        requires 0<= index < |ir|
+        requires 0<= index < |changes|
+        requires 0<= changes[index] < |p.commands|
+        requires forall d:: 0<= d < |changes| ==> 0<= changes[d] < |p.commands|
+        requires p.commands[changes[index]] == '['
+        requires matched_forall_loop(p, ir, changes, index)
+        requires ir[index] == Jump(dest, true)
+        ensures matched_command_with_ir(p, ir, index, changes)
+        ensures matched_forall_loop(p, ir, changes, index+1)
+    {}
+
+    lemma AndIsImplicationJumpBack(p: Program, ir: seq<Instr>, index: int, changes: seq<int>, dest: int)
+        requires valid_program(p)
+        requires changes == Changes(p)
+        requires 0<= index < |ir|
+        requires 0<= index < |changes|
+        requires 0<= changes[index] < |p.commands|
+        requires forall d:: 0<= d < |changes| ==> 0<= changes[d] < |p.commands|
+        requires p.commands[changes[index]] == ']'
+        requires matched_forall_loop(p, ir, changes, index)
+        requires ir[index] == Jump(dest, false)
+        ensures matched_command_with_ir(p, ir, index, changes)
+        ensures matched_forall_loop(p, ir, changes, index+1)
+    {}
+
+    lemma AndIsImplicationInput(p: Program, ir: seq<Instr>, index: int, changes: seq<int>)
+        requires valid_program(p)
+        requires changes == Changes(p)
+        requires 0<= index < |ir|
+        requires 0<= index < |changes|
+        requires 0<= changes[index] < |p.commands|
+        requires forall d:: 0<= d < |changes| ==> 0<= changes[d] < |p.commands|
+        requires p.commands[changes[index]] == ','
+        requires matched_forall_loop(p, ir, changes, index)
+        requires ir[index] == UserInput
+        ensures matched_command_with_ir(p, ir, index, changes)
+        ensures matched_forall_loop(p, ir, changes, index+1)
+    {}
+
+    lemma AndIsImplicationPrint(p: Program, ir: seq<Instr>, index: int, changes: seq<int>)
+        requires valid_program(p)
+        requires changes == Changes(p)
+        requires 0<= index < |ir|
+        requires 0<= index < |changes|
+        requires 0<= changes[index] < |p.commands|
+        requires forall d:: 0<= d < |changes| ==> 0<= changes[d] < |p.commands|
+        requires p.commands[changes[index]] == '.'
+        requires matched_forall_loop(p, ir, changes, index)
+        requires ir[index] == Print
+        ensures matched_command_with_ir(p, ir, index, changes)
+        ensures matched_forall_loop(p, ir, changes, index+1)
+    {}
+    lemma subtraction_equiv(p: Program, commands: seq<Instr>, k: int, j: int, next_command_indices: seq<int>)
+        requires valid_program(p)
+        requires next_command_indices == Changes(p)
+        requires 0<= k-1 < |next_command_indices|
+        requires 0<= k-1 < |commands|
+        requires 0<= next_command_indices[k-1] < |p.commands|
+        requires matched_command_with_ir(p, commands, k-1, next_command_indices)
+        requires j==k
+        ensures matched_command_with_ir(p, commands, j-1, next_command_indices)
+    {}
+
+    lemma ForAllStep2(p: Program, res: seq<int>)
+      requires changes_correct(p, res)
+      requires forall d:: 0 <= d < |res| ==> 0<= res[d] < |p.commands|
+      requires sub_changes(p, res)
+      ensures forall d:: (d in res && p.commands[d] in ['+', '-', '<', '>']) ==> next_step(p, d, count_consecutive_symbols(p, d), res)
+    {}
+
+    lemma AllLessThanLast(s: seq<int>)
+    requires |s| > 0 // Ensure the sequence is not empty
+    requires forall i, j :: 0 <= i < j < |s| ==> s[i] < s[j] // Strictly increasing
+    ensures forall i :: 0 <= i < |s| ==> s[i] <= s[|s| - 1] // All elements (except the last) are less than the last
+    {}
+
+    lemma AndElim(s: seq<int>, i: int, t: seq<int>)
+        requires forall k:: k in s ==> i> k && k in t
+        ensures forall k:: k in s ==> i > k
+    {}
+
+    lemma EquivStatement(s: seq<int>, s2: seq<int>)
+        requires forall k:: k in s ==> k in s2
+        ensures forall k:: int_in_seq(k, s) ==> int_in_seq(k, s2)
+    {} 
+
+    lemma AndIsImplicationPlus(p: Program, ir: seq<Instr>, index: int, changes: seq<int>, k: int)
+        requires valid_program(p)
+        requires changes == Changes(p)
+        requires 0<= index < |ir|
+        requires 0<= index < |changes|
+        requires 0<= changes[index] < |p.commands|
+        requires forall d:: 0<= d < |changes| ==> 0<= changes[d] < |p.commands|
+        requires ir[index] == Inc(k)
+        requires p.commands[changes[index]] == '+'
+        requires k == count_consecutive_symbols(p, changes[index])
+        requires k >= 0
+        requires ir[index] == Inc(k)
+        requires matched_forall_loop(p, ir, changes, index)
+        requires ir[index] == Inc(k)
+        ensures matched_command_with_ir(p, ir, index, changes)
+        ensures matched_forall_loop(p, ir, changes, index+1)
+    {}
+
+    lemma AndIsImplicationMinus(p: Program, ir: seq<Instr>, index: int, changes: seq<int>, k: int)
+        requires valid_program(p)
+        requires changes == Changes(p)
+        requires 0<= index < |ir|
+        requires 0<= index < |changes|
+        requires 0<= changes[index] < |p.commands|
+        requires forall d:: 0<= d < |changes| ==> 0<= changes[d] < |p.commands|
+        requires p.commands[changes[index]] == '-'
+        requires k == -1*count_consecutive_symbols(p, changes[index])
+        requires matched_forall_loop(p, ir, changes, index)
+        requires k < 0
+        requires ir[index] == Inc(k)
+        ensures matched_command_with_ir(p, ir, index, changes)
+        ensures matched_forall_loop(p, ir, changes, index+1)
+    {}
+
+    lemma AndIsImplicationMoveForwards(p: Program, ir: seq<Instr>, index: int, changes: seq<int>, k: int)
+        requires valid_program(p)
+        requires changes == Changes(p)
+        requires 0<= index < |ir|
+        requires 0<= index < |changes|
+        requires 0<= changes[index] < |p.commands|
+        requires p.commands[changes[index]] == '>'
+        requires k == count_consecutive_symbols(p, changes[index])
+        requires forall d:: 0<= d < |changes| ==> 0<= changes[d] < |p.commands|
+        requires matched_forall_loop(p, ir, changes, index)
+        requires k >= 0
+        requires ir[index] == Move(k)
+        ensures matched_command_with_ir(p, ir, index, changes)
+        ensures matched_forall_loop(p, ir, changes, index+1)
+    {}
+
+    lemma length_constraints(len: int, s1: seq<int>, s2: seq<int>)
+        requires len >= |s2|
+        requires len == |s1|
+        requires len <= |s2| && s1 == s2[..len]
+        ensures |s1| == |s2|
+    {}
+
+    lemma single_step_within_range(p: Program, i: int, k: int, next_command_indices: seq<int>)
+        requires k==1
+        requires next_command_indices == Changes(p)
+        requires 0<= i < |p.commands|
+        requires p.commands[i]==',' || p.commands[i] == '.' || p.commands[i] == '[' || p.commands[i] == ']'
+        requires changes_correct(p, next_command_indices)
+        ensures i in next_command_indices ==> next_step(p, i, k, next_command_indices)
+    {}
+
+
+}
